protocol framework

ironfleet/src/Dafny/Distributed/Protocol/Raft/DistributedSystem.i.dfy
@@ -3,9 +3,89 @@
 // This file defines prortocol of Raft
 //
 /////////////////////////////////////////////////////////////////////////////
+include "../../Common/Native/Io.s.dfy"
+include "../../Common/Framework/Environment.s.dfy"
+include "Config.i.dfy"
+include "Server.i.dfy"
+include "ServerScheduler.i.dfy"
+include "Types.i.dfy"
 
 module Raft__DistributedSystem_i {
 
 import opened Environment_s
+import opened Native__Io_s
+import opened Raft__Config_i
+import opened Raft__Server_i
+import opened Raft__ServerScheduler_i
+import opened Raft__Types_i
+
+
+datatype RaftState = RaftState(
+  config: RaftConfig,
+  environment:LEnvironment<EndPoint, RaftMessage>,
+  serverSchedulers:seq<RaftServerScheduler>
+)
+
+// Protocol-level init
+predicate RaftInit(s:RaftState, c:RaftConfig)
+{
+  && s.config == c
+  && WellFormedLRaftConfig(c)
+  && LEnvironment_Init(s.environment)
+  && |s.serverSchedulers| == |c.server_eps|
+  && (forall i:int :: 0 <= i < |s.serverSchedulers| ==> RaftServerSchedulerInit(s.serverSchedulers[i], RaftServerConfig(i, c)))
+  
+}
+
+// Protocol-level next
+// Here a next step can be:
+//  1. A host performing ios
+//    1.1. RaftNextServer
+//    1.2. RaftNextClient
+//  2. The environment
+//    2.1. deliver a packet
+//    2.2. time advancing
+//    2.3. do nothing
+// And `RaftNextCommon` is commonly used by all circumstances
+predicate RaftNextCommon(s:RaftState, s':RaftState)
+{
+  && |s.serverSchedulers| == |s.config.server_eps|
+  && s.serverSchedulers == s'.serverSchedulers
+  && s.config == s'.config
+  && LEnvironment_Next(s.environment, s'.environment)
+}
+predicate RaftNextServer(s:RaftState, s':RaftState, idx:int, ios:seq<RaftIo>)
+{
+  && RaftNextCommon(s, s')
+  && 0 <= idx < |s.serverSchedulers|
+  && s.environment.nextStep == LEnvStepHostIos(s.config.server_eps[idx], ios)
+  && s'.serverSchedulers == s.serverSchedulers[idx := s'.serverSchedulers[idx]]
+  && RaftServerSchedulerNext(s.serverSchedulers[idx], s'.serverSchedulers[idx], ios)
+}
+
+predicate RaftNextClient(s:RaftState, s':RaftState, ep:EndPoint, ios:seq<RaftIo>)
+{
+  && RaftNextCommon(s, s')
+  && s.environment.nextStep.LEnvStepHostIos?
+}
+
+predicate RaftNextEnvironment(s:RaftState, s':RaftState)
+{
+  // servers and config remain unchanged
+  && RaftNextCommon(s, s')
+  // only environment may change
+  && !s.environment.nextStep.LEnvStepHostIos?
+}
+
+predicate RaftNext(s:RaftState, s':RaftState)
+{
+  || (exists idx, ios :: RaftNextServer(s, s', idx, ios))
+  || (exists ep, ios :: RaftNextClient(s, s', ep, ios))
+  || RaftNextEnvironment(s, s')
+}
+
+
+
+
 
 }
