ironfleet/src/Dafny/Distributed/Protocol/Raft/Server.i.dfy
@@ -3,7 +3,145 @@
 // This file defines behaviours of a server
 //
 /////////////////////////////////////////////////////////////////////////////
+include "../../Common/Framework/Environment.s.dfy"
+include "../../Services/Raft/AppStateMachine.s.dfy"
+include "Config.i.dfy"
+include "Types.i.dfy"
 
 module Raft__Server_i {
+
+import opened Environment_s
+import opened AppStateMachine_s
+import opened Raft__Config_i
+import opened Raft__Types_i
+
+datatype RaftServer = RaftServer(
+  config:RaftServerConfig,
+  role:RaftRole,
+  // persistent state
+  currentTerm:int,
+  votedFor:int,
+  log:seq<AppRequest>,
+  // volatile state on all servers
+  commitIndex:int,
+  lastApplied:int,
+  // volatile state on leaders
+  nextIndex:map<int, int>,
+  matchIndex:map<int, int>,
+  // App
+  app:AppState
+)
+
+predicate RaftServerInit(server:RaftServer, config:RaftServerConfig) {
+  && server.config == config
+  && server.currentTerm == 0
+  && server.votedFor == -1
+  && server.log == []
+  && server.commitIndex == 0
+  && server.lastApplied == 0
+  && server.nextIndex == map []
+  && server.matchIndex == map []
+}
+
+predicate SpontaneousIos(ios:seq<RaftIo>, clocks:int)
+  requires 0<=clocks<=1
+{
+  && clocks <= |ios|
+  && (forall i :: 0<=i<clocks ==> ios[i].LIoOpReadClock?)
+  && (forall i :: clocks<=i<|ios| ==> ios[i].LIoOpSend?)
+}
+
+function SpontaneousClock(ios:seq<RaftIo>) : ClockReading
+{
+  if SpontaneousIos(ios, 1) then ClockReading(ios[0].t) else ClockReading(0) // nonsense to avoid putting a precondition on this function
+}
+
+predicate RaftServerNextHandleRequestVote(s:RaftServer, s':RaftServer, ios:seq<RaftIo>)
+{
+  true
+}
+
+predicate RaftServerNextHandleRequestVoteReply(s:RaftServer, s':RaftServer, ios:seq<RaftIo>)
+{
+  true
+}
+
+predicate RaftServerNextHandleAppendEntries(s:RaftServer, s':RaftServer, ios:seq<RaftIo>)
+{
+  true
+}
+
+predicate RaftServerNextHandleAppendEntriesReply(s:RaftServer, s':RaftServer, ios:seq<RaftIo>)
+{
+  true
+}
+
+predicate RaftServerNextProcessPacket(s:RaftServer, s':RaftServer, ios:seq<RaftIo>)
+{
+  && |ios| >= 1
+  && if ios[0].LIoOpTimeoutReceive? then
+      s' == s && |ios| == 1 // TODO: why?
+    else
+      (
+        && ios[0].LIoOpReceive?
+        && if ios[0].r.msg.RequestVote? then
+            RaftServerNextHandleRequestVote(s, s', ios)
+          else if ios[0].r.msg.RequestVoteReply? then
+            RaftServerNextHandleRequestVoteReply(s, s', ios)
+          else if ios[0].r.msg.AppendEntries? then
+            // Note: this is the only one that may requires a election timeout reset
+            RaftServerNextHandleAppendEntries(s, s', ios)
+          else 
+            ios[0].r.msg.AppendEntriesReply? && RaftServerNextHandleAppendEntriesReply(s, s', ios)
+      )
+}
+
+function {:opaque} ExtractSentPacketsFromIos(ios:seq<RaftIo>) : seq<RaftPacket>
+  ensures forall p :: p in ExtractSentPacketsFromIos(ios) <==> LIoOpSend(p) in ios
+{
+  if |ios| == 0 then
+    []
+  else if ios[0].LIoOpSend? then
+    [ios[0].s] + ExtractSentPacketsFromIos(ios[1..])
+  else
+    ExtractSentPacketsFromIos(ios[1..])
+}
+
+predicate RaftServerNextReadClockMaybeSendHeartbeat(s:RaftServer, s':RaftServer, clock:ClockReading, sent_packets:seq<RaftPacket>)
+{
+  true
+}
+
+predicate RaftServerNextReadClockMaybeStartElection(s:RaftServer, s':RaftServer, clock:ClockReading, sent_packets:seq<RaftPacket>)
+{
+  true
+}
+
+predicate RaftServerNoReceiveNext(s:RaftServer, nextActionIndex:int, s':RaftServer, ios:seq<RaftIo>)
+{
+  var sent_packets := ExtractSentPacketsFromIos(ios);
+
+  if nextActionIndex == 1 then
+    if s.role.Leader? then
+      // leader may timeout for heartbeat
+      && SpontaneousIos(ios, 1)
+      && RaftServerNextReadClockMaybeSendHeartbeat(s, s', SpontaneousClock(ios), sent_packets)
+    else if s.role.Follower? then
+      // follower may timeout for election
+      && SpontaneousIos(ios, 1)
+      && RaftServerNextReadClockMaybeStartElection(s, s', SpontaneousClock(ios), sent_packets)
+    else
+      //candidate may timeout for election
+      && s.role.Candidate?
+      && SpontaneousIos(ios, 1)
+      && RaftServerNextReadClockMaybeStartElection(s, s', SpontaneousClock(ios), sent_packets)
+  else
+    false
+}
+
+function RaftServerNumActions() : int
+{
+  10
+}
 
 }
