ironfleet/src/Dafny/Distributed/Protocol/Raft/Config.i.dfy
@@ -1,0 +1,50 @@
+include "Types.i.dfy"
+include "../../Common/Collections/Sets.i.dfy"
+include "../../Common/Collections/Seqs.i.dfy"
+
+module Raft__Config_i {
+import opened Raft__Types_i
+import opened Native__Io_s
+import opened Collections__Sets_i
+import opened Collections__Seqs_i
+
+datatype RaftConfig = RaftConfig(
+  client_eps:set<EndPoint>,
+  server_eps:seq<EndPoint>,
+  min_election_timeout:int,
+  max_election_timeout:int,
+  heartbeat_timeout:int
+  )
+
+datatype RaftServerConfig = RaftServerConfig(
+  server_id:int,
+  global_config:RaftConfig
+)
+
+function RaftMinQuorumSize(c:RaftConfig) : int
+{
+  |c.server_eps|/2+1
+}
+
+predicate ReplicasDistinct(server_eps:seq<EndPoint>, i:int, j:int)
+{
+  0 <= i < |server_eps| && 0 <= j < |server_eps| && server_eps[i] == server_eps[j] ==> i == j
+}
+
+function WellFormedLRaftConfig(c:RaftConfig) : bool
+{
+  && |c.server_eps| > 0
+  && c.min_election_timeout > 0
+  && c.max_election_timeout > 0
+  && c.min_election_timeout < c.max_election_timeout
+  && c.heartbeat_timeout > 0
+  && forall i,j :: ReplicasDistinct(c.server_eps, i, j)
+}
+
+function WellFormedLRaftServerConfig(c:RaftServerConfig) : bool
+{
+  && WellFormedLRaftConfig(c.global_config)
+  && 0 <= c.server_id
+}
+
+} 
