ironfleet/src/Dafny/Distributed/Protocol/Raft/ServerScheduler.i.dfy
@@ -1,0 +1,32 @@
+include "Config.i.dfy"
+include "Server.i.dfy"
+include "Types.i.dfy"
+
+module Raft__ServerScheduler_i {
+
+import opened Raft__Config_i
+import opened Raft__Server_i
+import opened Raft__Types_i
+
+datatype RaftServerScheduler = RaftServerScheduler(
+  server:RaftServer,
+  nextActionIndex:int
+)
+
+predicate RaftServerSchedulerInit(sch:RaftServerScheduler, c:RaftServerConfig) 
+  requires WellFormedLRaftServerConfig(c)
+{
+  && RaftServerInit(sch.server, c)
+  && sch.nextActionIndex == 0
+}
+
+predicate RaftServerSchedulerNext(sch:RaftServerScheduler, sch':RaftServerScheduler, ios:seq<RaftIo>) 
+{
+  && sch'.nextActionIndex == (sch.nextActionIndex + 1) % RaftServerNumActions()
+  && if sch.nextActionIndex == 0 then
+      RaftServerNextProcessPacket(sch.server, sch'.server, ios)
+    else
+      RaftServerNoReceiveNext(sch.server, sch.nextActionIndex, sch'.server, ios)
+
+}
+}
